---
"course:": "[[DMath]]"
"tags:":
---
| A | B | A$\rightarrow$B | A$\wedge$(A$\rightarrow$B) | (A$\wedge$(A$\rightarrow$B)) $\rightarrow$ B |
|---|---|-----------------|----------------------------|---|
| 0 | 0 | 1               | 0                          | 1 |
| 0 | 1 | 1               | 0                          | 1 |
| 1 | 0 | 0               | 0                          | 1 |
| 1 | 1 | 1               | 1                          | 1 |

>man kann S beweisen, indem
>	1. eine Aussage R formulieren
>	2. R beweisen
>	3. R$\Rightarrow$S beweisen
>
>A$\wedge$(A$\rightarrow$B) $\models$ B

> [!example] Lemma 2.1
> 





